# Sommatorie
- $\sum\limits_{i = 1}^{n} {i}=$ $\dfrac{(n+1) · n}{2} \Longrightarrow θ(n^2)$

- $\sum\limits_{i = 1}^{n-1} {i}= \sum\limits_{i = 2}^{n} {i-1} =$   $\dfrac{(n-1) · n}{2} \Longrightarrow θ(n^2)$

- $\sum\limits_{i = 1}^{n} {i^2}=$   $\dfrac{n · (n+1) · (2n+1)}{2} \Longrightarrow θ(n^3)$

- $\sum\limits_{i = 1}^{n-1} {n-i}=$  $\sum\limits_{i = 1}^{n-1} {i} \Longrightarrow θ(n^2)$
***
- $\sum\limits_{k = 0}^{∞} {x^k} = \dfrac{1}{1-x}$ con $|x|<1$

- $\sum\limits_{k = 0}^{∞} {k·x^k} = \dfrac{x}{(1-x)^2}$ con $|x|<1$
